steel/Zeta.Steel.SafeMain.fsti
@@ -10,17 +10,18 @@ module A = Steel.ST.Array
 module AT = Zeta.Steel.ApplicationTypes
 module EXT = Zeta.Steel.ExternalPtr
 module U16 = FStar.UInt16
+module TSM = Zeta.Steel.ThreadStateModel
 
 open Steel.ST.Util
 
 val handle_pts_to
-  (ts: M.top_level_state)
+  (ts: M.top_level_state false)
 : Tot vprop
 
 val gather
   (#opened: _)
-  (ts1: M.top_level_state)
-  (ts2: M.top_level_state)
+  (ts1: M.top_level_state false)
+  (ts2: M.top_level_state false)
 : STGhost unit opened
     (handle_pts_to ts1 `star` handle_pts_to ts2)
     (fun _ -> handle_pts_to ts1)
@@ -29,7 +30,7 @@ val gather
 
 val share
   (#opened: _)
-  (ts: M.top_level_state)
+  (ts: M.top_level_state false)
 : STGhostT unit opened
     (handle_pts_to ts)
     (fun _ -> handle_pts_to ts `star` handle_pts_to ts)
@@ -59,6 +60,21 @@ let check_verify_input
   EXT.valid input len &&
   EXT.valid output out_len
 
+let verify_post_success_pure_inv
+  (tid:AT.tid)
+  (log_bytes:Ghost.erased AT.bytes)
+  (out_bytes:Ghost.erased AT.bytes)
+  (read wrote:U32.t)  
+  (out_bytes':Seq.seq U8.t)
+  : prop
+  =
+    (exists (entries entries': AEH.log) . (
+      let tsm = TSM.verify_model (TSM.init_thread_state_model tid) entries in
+     let tsm' = TSM.verify_model tsm entries' in
+     Log.parse_log_up_to log_bytes (U32.v read) == Some entries' /\
+     Application.n_out_bytes tsm tsm' 0ul wrote out_bytes out_bytes'
+    ))
+
 [@@__reduce__]
 let verify_post_some_m_success_body
   (tid:U16.t)
@@ -69,25 +85,21 @@ let verify_post_some_m_success_body
   (out_len: U32.t)
   (out_bytes: AT.bytes)
   (output: EXT.extern_ptr)
-  (v: option (v:V.verify_result { V.verify_result_complete len v }))
+  (v: option (M.verify_result len))
   (sq: squash (check_verify_input tid len input out_len output))
-  (t: M.top_level_state)
-  (entries: _)
+  (t: M.top_level_state false)
   (read:U32.t)
   (wrote:U32.t)
-  (entries' : _)
   (out_bytes' : _)
 : Tot vprop
 =        A.pts_to (EXT.gtake output) full_perm out_bytes'
            `star`
-         pure (M.verify_post_success_pure_inv
+         pure (verify_post_success_pure_inv
             tid
-            entries
             log_bytes
             out_bytes
             read
             wrote
-            entries'
             out_bytes')
 
 [@@__reduce__]
@@ -100,16 +112,16 @@ let verify_post_some_m_success
   (out_len: U32.t)
   (out_bytes: AT.bytes)
   (output: EXT.extern_ptr)
-  (v: option (v:V.verify_result { V.verify_result_complete len v }))
+  (v: option (M.verify_result len))
   (sq: squash (check_verify_input tid len input out_len output))
-  (t: M.top_level_state)
+  (t: M.top_level_state false)
   (read:U32.t)
   (wrote:U32.t)
 : Tot vprop
 =
-       exists_ (fun entries -> exists_ (fun entries' -> exists_ (fun out_bytes' ->
-         verify_post_some_m_success_body tid log_perm log_bytes len input out_len out_bytes output v sq t entries read wrote entries' out_bytes'
-       )))
+       exists_ (fun out_bytes' ->
+         verify_post_some_m_success_body tid log_perm log_bytes len input out_len out_bytes output v sq t read wrote out_bytes'
+       )
 
 [@@__reduce__]
 let verify_post_some_m_failure
@@ -127,7 +139,7 @@ let verify_post_some_m
   (out_bytes: AT.bytes)
   (output: EXT.extern_ptr)
   (v: option (v:V.verify_result { V.verify_result_complete len v }))
-  (t: M.top_level_state)
+  (t: M.top_level_state false)
 : Tot vprop
 = match v with
   | Some (V.Verify_success read wrote) ->
@@ -166,7 +178,7 @@ let verify_post
   (out_len: U32.t)
   (out_bytes: AT.bytes)
   (output: EXT.extern_ptr)
-  (res: option (v:V.verify_result { V.verify_result_complete len v }))
+  (res: option (M.verify_result len))
 : Tot vprop
 = verify_post_some tid log_perm log_bytes len input out_len out_bytes output res
 
@@ -179,7 +191,7 @@ val verify_log
                (out_len: U32.t)
                (#out_bytes:Ghost.erased AT.bytes)
                (output: EXT.extern_ptr)
-  : STT (option (v:V.verify_result { V.verify_result_complete len v }))
+  : STT (option (M.verify_result len))
     (verify_pre log_perm log_bytes input out_bytes output)
     (fun res -> verify_post tid log_perm log_bytes len input out_len out_bytes output res)
 
